examples/map/MapA.v
@@ -9,6 +9,8 @@ Require Import PCM.
 Require Import HoareDef STB IPM.
 Require Import MapHeader.
 
+Require Import sProp sWorld World SRF.
+
 Set Implicit Arguments.
 
 
@@ -29,8 +31,9 @@ def set_by_user(k: int) ≡
 ***)
 
 Section A.
-  Context `{@GRA.inG MapRA0 Σ}.
-  Context `{@GRA.inG MapRA1 Σ}.
+  Context `{_W: CtxWD.t}.
+  Context `{@GRA.inG MapRA Γ}.
+  Context `{@GRA.inG MapRA0 Γ}.
 
   (* Let Es := (hAPCE +' Es). *)
 
@@ -70,7 +73,7 @@ Section A.
 
   Definition SMapSem: SModSem.t := {|
     SModSem.fnsems := MapSbtb;
-    SModSem.initial_cond := Own (GRA.embed (Excl.unit, Auth.excl ((fun _ => Excl.just 0%Z): @URA.car (Z ==> (Excl.t Z))%ra) ((fun _ => Excl.just 0%Z): @URA.car (Z ==> (Excl.t Z))%ra)));
+    SModSem.initial_cond := OwnM (Excl.unit, Auth.excl ((fun _ => Excl.just 0%Z): @URA.car (Z ==> (Excl.t Z))%ra) ((fun _ => Excl.just 0%Z): @URA.car (Z ==> (Excl.t Z))%ra));
     (* SModSem.initial_mr := GRA.embed (Excl.unit, Auth.excl ((fun _ => Excl.just 0%Z): @URA.car (Z ==> (Excl.t Z))%ra) ((fun _ => Excl.just 0%Z): @URA.car (Z ==> (Excl.t Z))%ra)); *)
     SModSem.initial_st := Ret (fun (_: Z) => 0%Z)↑;
   |}
